A decomposition lemma for region_addrs

theories/region.v
@@ -1,31 +1,307 @@
 From cap_machine Require Export lang rules.
 From iris.proofmode Require Import tactics.
+(*Require Import Coq.Program.Wf.*)
 
 Section region.
   Context `{memG Σ, regG Σ}.
 
-  Fixpoint region_addrs (b e : Addr) (n : nat) {struct n} : list Addr :=
+  (* Not usable without proving some sort of rewriting rule, and can't manage to prove it *)
+  (* Program Fixpoint region_addrs (b e: Addr) { measure (Z.to_nat (e - b)%Z) }: list Addr := *)
+  (*   if Z.eq_dec b e then b::nil else *)
+  (*     if Z_lt_dec b e then  *)
+  (*       match (b + 1)%a with *)
+  (*       | Some b' => b::region_addrs b' e *)
+  (*       | None => False_rect _ _  *)
+  (*       end *)
+  (*     else nil. *)
+  (* Next Obligation. *)
+  (*   intros. unfold incr_addr in *. *)
+  (*   destruct (Z_le_dec (b + 1)%Z MemNum); try discriminate. *)
+  (*   inv Heq_anonymous. simpl. destruct e; simpl. *)
+  (*   destruct b; simpl in *. assert (z - z0 = Z.succ (z - (z0 + 1)))%Z by omega. *)
+  (*   rewrite H3. rewrite Z2Nat.inj_succ; omega. Defined. *)
+  (* Next Obligation. *)
+  (*   intros. unfold incr_addr in *. *)
+  (*   destruct (Z_le_dec (b + 1)%Z MemNum); try discriminate. *)
+  (*   destruct b; destruct e; simpl in *. *)
+  (*   apply Z.leb_le in fin. apply Z.leb_le in fin0. *)
+  (*   omega. Defined. *)
+  (* Next Obligation. apply measure_wf. apply lt_wf. Defined. *)
+
+  Fixpoint region_addrs_aux (b: Addr) (n: nat): list Addr :=
+    match n with
+    | 0 => nil
+    | S n => b :: (region_addrs_aux (get_addr_from_option_addr (b + 1)%a) n)
+    end.
+
+  Lemma region_addrs_aux_length:
+    forall n b,
+      length (region_addrs_aux b n) = n.
+  Proof. induction n; intros; simpl; auto. Qed.
+
+  Lemma region_addrs_aux_decomposition:
+    forall n b k,
+      (k <= n)%nat ->
+      region_addrs_aux b n = region_addrs_aux b k ++ (region_addrs_aux (get_addr_from_option_addr (b + Z.of_nat k)%a) (n - k)).
+  Proof.
+    induction n; intros.
+    - assert ((k = 0)%nat) by Lia.lia; subst k.
+      reflexivity.
+    - inv H1.
+      + rewrite Nat.sub_diag. simpl.
+        rewrite app_nil_r. auto.
+      + simpl. destruct k; simpl.
+        * assert (b = get_addr_from_option_addr (b + 0%nat)%a).
+          { destruct b; unfold incr_addr; simpl.
+            generalize (Zle_bool_imp_le _ _ fin). intro Y.
+            destruct (Z_le_dec (z + 0%nat)%Z MemNum); try Lia.lia.
+            simpl. apply z_of_eq; simpl. Lia.lia. }
+          rewrite <- H1. reflexivity.
+        * generalize (IHn (get_addr_from_option_addr (b + 1)%a) k ltac:(omega)). intros A.
+          rewrite A. do 3 (f_equal; auto). destruct b; unfold incr_addr; simpl.
+          generalize (Zle_bool_imp_le _ _ fin). intro Y.
+          destruct (Z_le_dec (z + 1)%Z MemNum); simpl.
+          { destruct (Z_le_dec (z + 1 + k)%Z MemNum); simpl.
+            - destruct (Z_le_dec (z + S k)%Z MemNum); simpl.
+              + apply z_of_eq; simpl. Lia.lia.
+              + elim n0. Lia.lia.
+            - destruct (Z_le_dec (z + S k)%Z MemNum); simpl.
+              + elim n0. Lia.lia.
+              + reflexivity. }
+          { assert (z = MemNum) by Lia.lia. subst z.
+            destruct (Z_le_dec (MemNum + S k)%Z MemNum).
+            - exfalso. Lia.lia.
+            - simpl. destruct (Z_le_dec (MemNum + k)%Z MemNum); simpl; auto.
+              apply z_of_eq. simpl. Lia.lia. }
+  Qed.
+
+  Lemma region_addrs_aux_spec:
+    forall n b k,
+      (k < n)%nat ->
+      nth_error (region_addrs_aux b n) k = Some (get_addr_from_option_addr (b + (Z.of_nat k))%a).
+  Proof.
+    induction n; intros.
+    - inv H1.
+    - assert (X: k = n \/ k < n) by omega; destruct X as [X | X].
+      + subst k. simpl. destruct n.
+        * simpl. f_equal.
+          unfold incr_addr; destruct b; simpl.
+          generalize (Zle_bool_imp_le _ _ fin). intro Y.
+          destruct (Z_le_dec (z + 0%nat)%Z MemNum); try omega.
+          { simpl. apply z_of_eq; simpl. rewrite Z.add_0_r. reflexivity. }
+          { elim n. rewrite Z.add_0_r. exact Y. }
+        * replace (nth_error (b :: region_addrs_aux (get_addr_from_option_addr (b + 1)%a) (S n)) (S n)) with (nth_error (region_addrs_aux (get_addr_from_option_addr (b + 1)%a) (S n)) n) by reflexivity.
+          rewrite IHn; try omega.
+          f_equal. unfold incr_addr; destruct b; simpl.
+          generalize (Zle_bool_imp_le _ _ fin). intro Y.
+          destruct (Z_le_dec (z + 1)%Z MemNum).
+          { simpl. f_equal. assert (Z: (z + 1 + n)%Z = (z + S n)%Z) by (rewrite Nat2Z.inj_succ; omega).
+            destruct (Z_le_dec (z + 1 + n)%Z MemNum); destruct (Z_le_dec (z + S n)%Z MemNum); try omega; auto.
+            f_equal. apply z_of_eq. simpl.
+            rewrite Nat2Z.inj_succ. omega. }
+          { assert (z = MemNum) by omega. subst z. simpl.
+            rewrite Nat2Z.inj_succ.
+            destruct (Z_le_dec (MemNum + Z.succ n)%Z MemNum); try omega.
+            simpl. destruct (Z_le_dec (MemNum + n)%Z MemNum).
+            - simpl. apply z_of_eq. simpl. omega.
+            - simpl. reflexivity. }
+      + rewrite <- IHn; auto.
+        generalize (region_addrs_aux_decomposition (S n) b n ltac:(omega)).
+        intros A. rewrite A.
+        rewrite nth_error_app1; auto.
+        rewrite region_addrs_aux_length. auto.
+  Qed.
+
+  Definition region_addrs (b e: Addr): list Addr :=
+    if Z_le_dec b e then region_addrs_aux b (region_size b e) else nil.
+
+  Lemma region_addrs_length:
+    forall b e,
+      (b <= e)%a ->
+      length (region_addrs b e) = region_size b e.
+  Proof.
+    intros; unfold region_addrs.
+    destruct (Z_le_dec b e).
+    - apply region_addrs_aux_length.
+    - elim n. exact H1.
+  Qed.
+
+  Lemma region_addrs_spec:
+    forall b e k,
+      (b <= e)%a ->
+      (k < region_size b e)%nat ->
+      nth_error (region_addrs b e) k = Some (get_addr_from_option_addr (b + (Z.of_nat k))%a).
+  Proof.
+    intros; unfold region_addrs.
+    destruct (Z_le_dec b e).
+    - apply region_addrs_aux_spec; auto.
+    - elim n. exact H1.
+  Qed.
+
+  Lemma list_nth_eq:
+    forall A (l1 l2: list A),
+      (forall n, nth_error l1 n = nth_error l2 n) ->
+      l1 = l2.
+  Proof.
+    induction l1; intros.
+    - destruct l2; auto.
+      generalize (H1 0). simpl. discriminate.
+    - destruct l2.
+      + generalize (H1 0); simpl; discriminate.
+      + generalize (H1 0); simpl; intros.
+        inv H2. f_equal.
+        apply IHl1. intros.
+        generalize (H1 (S n)); simpl; auto.
+  Qed.
+  
+  Lemma addr_conv:
+    forall (b a: Addr),
+      (b + (a - b)%Z)%a = Some a.
+  Proof.
+    intros. unfold incr_addr; destruct a; destruct b; simpl.
+    generalize (Zle_bool_imp_le _ _ fin). generalize (Zle_bool_imp_le _ _ fin0). intros A B.
+    destruct (Z_le_dec (z0 + (z - z0))%Z MemNum); try omega.
+    f_equal. apply z_of_eq; simpl. omega.
+  Qed.
+
+  Lemma region_addrs_decomposition:
+    forall b a e,
+      (b <= a /\ a <= e)%a ->
+      region_addrs b e = region_addrs b (get_addr_from_option_addr (a + (-1))%a)
+                         ++ (a :: match (a + 1)%a with
+                                  | Some y => region_addrs y e
+                                  | _ => nil
+                                  end).
+  Proof.
+    intros. unfold region_addrs at 1.
+    assert (b <= e)%Z by (unfold le_addr in H1; omega).
+    destruct (Z_le_dec b e); try omega.
+    assert (X: length (region_addrs b (get_addr_from_option_addr (a + -1)%a)) <= region_size b e).
+    { unfold region_addrs. destruct (Z_le_dec b (get_addr_from_option_addr (a + -1)%a)).
+      - rewrite region_addrs_aux_length. unfold region_size.
+        apply le_n_S. apply Zabs_nat_le; split.
+        + omega.
+        + destruct a; destruct b; destruct e; unfold incr_addr; unfold le_addr in *; simpl in *.
+          generalize (Zle_bool_imp_le _ _ fin). intro X1.
+          destruct (Z_le_dec (z + -1)%Z MemNum); try omega.
+          simpl. omega.
+      - simpl; Lia.lia. }
+    erewrite region_addrs_aux_decomposition; eauto. f_equal.
+    { unfold region_addrs.
+      destruct (Z_le_dec b (get_addr_from_option_addr (a + -1)%a)).
+      - rewrite region_addrs_aux_length. reflexivity.
+      - reflexivity. }
+    assert ((get_addr_from_option_addr (b + length (region_addrs b (get_addr_from_option_addr (a + -1))))%a) = a).
+    { unfold region_addrs. destruct (Z_le_dec b (get_addr_from_option_addr (a + -1)%a)).
+      - rewrite region_addrs_aux_length.
+        unfold region_size; destruct b; destruct a; unfold le_addr in *; unfold incr_addr in *; simpl in *.
+        generalize (Zle_bool_imp_le _ _ fin). intro X1.
+        generalize (Zle_bool_imp_le _ _ fin0). intro X2.
+        destruct (Z_le_dec (z0 + -1)%Z MemNum); try omega.
+        simpl. destruct H1.
+        assert ((z + S (Z.abs_nat (z0 + -1 - z)))%Z = z0).
+        { simpl in l0. Lia.lia. }
+        destruct (Z_le_dec (z + S (Z.abs_nat (z0 + -1 - z)))%Z MemNum); try omega.
+        simpl. apply z_of_eq; auto.
+      - simpl. destruct b; destruct a; unfold le_addr in *; unfold incr_addr in *; simpl in *.
+        generalize (Zle_bool_imp_le _ _ fin). intro X1.
+        generalize (Zle_bool_imp_le _ _ fin0). intro X2.
+        destruct (Z_le_dec (z + 0%nat)%Z MemNum); try Lia.lia.
+        simpl. apply z_of_eq; simpl. destruct (Z_le_dec (z0 + -1)%Z MemNum); try omega.
+        simpl in n. Lia.lia. }
+    rewrite H3.
+    assert ((region_size b e - length (region_addrs b (get_addr_from_option_addr (a + -1)%a))) = S (length (match (a + 1)%a with
+       | Some y => region_addrs y e
+       | None => []
+       end))).
+    { unfold region_addrs. destruct (Z_le_dec b (get_addr_from_option_addr (a + -1)%a)).
+      - rewrite region_addrs_aux_length. case_eq (a + 1)%a; intros.
+        + destruct (Z_le_dec a0 e).
+          * rewrite region_addrs_aux_length.
+            unfold region_size; destruct b; destruct a; destruct e; unfold le_addr in *; unfold incr_addr in *; simpl in *.
+            generalize (Zle_bool_imp_le _ _ fin). intro X1.
+            generalize (Zle_bool_imp_le _ _ fin0). intro X2.
+            generalize (Zle_bool_imp_le _ _ fin1). intro X3.
+            destruct (Z_le_dec (z0 + -1)%Z MemNum); try omega; simpl in *.
+            destruct (Z_le_dec (z0 + 1)%Z MemNum); inv H4; simpl in *.
+            repeat (rewrite Zabs2Nat.abs_nat_nonneg; try omega).
+            rewrite <- Z2Nat.inj_sub; try omega.
+            replace (z1 - z - (z0 + -1 - z))%Z with (z1 - z0 + 1)%Z by omega.
+            do 2 (rewrite <- Z2Nat.inj_succ; try omega).
+            f_equal; omega.
+          * destruct H1; unfold region_size; destruct b; destruct a; destruct e; unfold le_addr in *; unfold incr_addr in *; simpl in *.
+            generalize (Zle_bool_imp_le _ _ fin). intro X1.
+            generalize (Zle_bool_imp_le _ _ fin0). intro X2.
+            generalize (Zle_bool_imp_le _ _ fin1). intro X3.
+            destruct (Z_le_dec (z0 + -1)%Z MemNum); try omega; simpl in *.
+            destruct (Z_le_dec (z0 + 1)%Z MemNum); inv H4; simpl in *.
+            assert (z0 = z1) by omega. subst z0.
+            repeat (rewrite Zabs2Nat.abs_nat_nonneg; try omega).
+            rewrite <- Z2Nat.inj_sub; try omega.
+            replace ((z1 - z - (z1 + -1 - z))%Z) with 1%Z by omega.
+            reflexivity.
+        + simpl. generalize (incr_addr_one_none _ H4). intro; subst a.
+          unfold addr_reg.top in *. destruct e; destruct b; unfold le_addr in *; unfold incr_addr in *; simpl in *.
+          generalize (Zle_bool_imp_le _ _ fin). intro X1.
+          generalize (Zle_bool_imp_le _ _ fin0). intro X2.
+          destruct H1. assert (z = MemNum) by omega. subst z.
+          repeat (rewrite Zabs2Nat.abs_nat_nonneg; try omega).
+          rewrite <- Z2Nat.inj_sub; try omega.
+          assert (MemNum - z0 - (MemNum + -1 - z0) = 1)%Z by omega.
+          rewrite H6. reflexivity.
+      - simpl. assert (a = b).
+        { destruct H1. destruct a; destruct b; unfold le_addr in *; unfold incr_addr in *; simpl in *.
+          generalize (Zle_bool_imp_le _ _ fin). intro X1.
+          generalize (Zle_bool_imp_le _ _ fin0). intro X2.
+          apply z_of_eq; simpl.
+          destruct (Z_le_dec (z + -1)%Z MemNum); try omega.
+          simpl in n. omega. } subst a. case_eq (b + 1)%a; intros.
+        + destruct (Z_le_dec a e).
+          * simpl. rewrite region_addrs_aux_length.
+            destruct H1. destruct e; destruct b; unfold le_addr in *; unfold incr_addr in *; simpl in *.
+            generalize (Zle_bool_imp_le _ _ fin). intro X1.
+            generalize (Zle_bool_imp_le _ _ fin0). intro X2.
+            destruct (Z_le_dec (z0 + 1)%Z MemNum); try congruence. inv H4. simpl.
+            f_equal. simpl in l0. rewrite <- Zabs2Nat.inj_succ; try omega.
+            f_equal. omega.
+          * simpl. destruct b; destruct a; destruct e; unfold le_addr in *; unfold incr_addr in *; simpl in *.
+          generalize (Zle_bool_imp_le _ _ fin). intro X1.
+          generalize (Zle_bool_imp_le _ _ fin0). intro X2.
+          generalize (Zle_bool_imp_le _ _ fin1). intro X3.
+          destruct (Z_le_dec (z + 1)%Z MemNum); try congruence.
+          inv H4. assert (z1 = z) by omega. subst z1. Lia.lia.
+        + simpl. generalize (incr_addr_one_none _ H4). intro; subst b.
+          unfold addr_reg.top in *. destruct H1; destruct e; unfold le_addr in *; unfold incr_addr in *; simpl in *.
+          generalize (Zle_bool_imp_le _ _ fin). intro X1.
+          assert (z = MemNum) by omega; subst z. Lia.lia. }
+    rewrite H4. simpl. f_equal.
+    unfold region_addrs. destruct (a + 1)%a.
+    { simpl. destruct (Z_le_dec a0 e); simpl; auto.
+      rewrite region_addrs_aux_length. reflexivity. }
+    { simpl. auto. }
+  Qed.
+
+
+
+  (*Fixpoint region_addrs (b e : Addr) (n : nat) {struct n} : list Addr :=
     if (b <=? e)%a && ((region_size b e) =? n)%nat then
       match n with
       | 0 => [b]
       | S n => b :: (region_addrs (get_addr_from_option_addr (b + 1)%a) e n)
       end
-    else [].
+    else [].*)
 
   Definition region_mapsto (b e : Addr) (ws : list Word) : iProp Σ :=
-    ([∗ list] k↦y1;y2 ∈ (region_addrs b e (region_size b e));ws, y1 ↦ₐ y2)%I. 
+    ([∗ list] k↦y1;y2 ∈ (region_addrs b e);ws, y1 ↦ₐ y2)%I. 
   
-
   Definition included (b' e' : Addr) (b e : Addr) : iProp Σ :=
     (⌜(b <= b')%a⌝ ∧ (⌜e' <= e⌝)%a)%I.
   
-
   Fixpoint in_range (a b e : Addr) : iProp Σ :=
     (⌜(b <= a)%a⌝ ∧ ⌜(a < e)%a⌝)%I.
 
-  Fixpoint region_mapsto_sub (b e : Addr) ws : iProp Σ := 
-    ([∗ list] k↦y1;y2 ∈ (region_addrs b e (region_size b e));take (region_size b e) ws,
-                                                             y1 ↦ₐ y2)%I. 
+  (* Fixpoint region_mapsto_sub (b e : Addr) ws : iProp Σ :=  *)
+  (*   ([∗ list] k↦y1;y2 ∈ (region_addrs b e);take (region_size b e) ws, y1 ↦ₐ y2)%I.  *)
 
   Lemma extract_from_region b e a ws φ : 
     (b <= a ∧ a <= e)%a →
@@ -37,22 +313,8 @@ Section region.
         ∗ a ↦ₐ w ∗ φ w
         ∗ region_mapsto ah e (drop (region_size b a) ws)
         ∗ ([∗ list] w ∈ (drop (region_size b a) ws), φ w))%I.
-  Proof. Admitted.  
-  
-  Lemma extract_from_region' b e a al ws φ :  
-    (b <= a ∧ a <= e)%a →
-    (a + -1)%a = Some al →
-    (region_mapsto b e ws ∗ ([∗ list] w ∈ ws, φ w)  ⊣⊢
-     (∃ w, region_mapsto b al (take (region_size b al) ws)
-        ∗ ([∗ list] w ∈ (take (region_size b al) ws), φ w) 
-        ∗ a ↦ₐ w ∗ φ w
-        ∗ match (a + 1)%a with
-          | Some ah => region_mapsto ah e (drop (region_size b a) ws)
-                      ∗ ([∗ list] w ∈ (drop (region_size b a) ws), φ w)
-          | None => True
-          end))%I.
-  Proof. Admitted. 
-
+  Proof. Admitted.
+    
   (* Lemma extract_from_region b e a al ah ws φ :   *)
   (*   (b <= a ∧ a <= e)%a → *)
   (*   (a + (Zneg 1))%a = Some al → *)
